\clearpage

\section{Safe $\lambda$-calculus without the homogeneity constraint}
\label{sec:safe_nonhomog}


In section \ref{sec:safe_homog}, we have presented a safe lambda
calculus in the setting of homogeneous types. In this section, we
give a general notion of safety for the simply typed
$\lambda$-calculus. The rules we give here do not assume homogeneity
of the types.

We call safe terms the simply typed lambda terms that are
typable within the following system of formation rules:

\subsection{Rules}

We use a set of sequents of the form $\Gamma \vdash M : A$ where $\Gamma$ is the context of the term and $A$ is its type.
The following system of rules defined the non homogeneous safe $\lambda$-calculus:

$$ \rulename{var} \quad  \rulef{}{x : A\vdash x : A}
\qquad  \rulename{const} \quad  \rulef{}{\vdash f : A} \quad f \in \Sigma, \ord{f} \leq 1
\qquad  \rulename{wk} \quad  \rulef{\Gamma \vdash M : A}{\Delta \vdash M : A} \quad \Sigma \subseteq \Gamma$$

$$ \rulename{app} \rulef{\Gamma \vdash M : (A,\ldots,A_l,B)
                                        \qquad \Gamma \vdash N_1 : A_1
                                        \quad \ldots \quad \Gamma \vdash N_l : A_l  }
                                   {\Gamma  \vdash M N_1 \ldots N_l : B}
                                    \quad
                                   \forall y \in \Gamma : \ord{y} \geq \ord{B}$$

$$ \rulename{abs} \quad  \rulef{\Gamma \union \overline{x} : \overline{A} \vdash M : B}
                                   {\Gamma  \vdash \lambda \overline{x} : \overline{A} . M : (\overline{A},B)} \qquad
                                   \forall y \in \Gamma : \ord{y} \geq \ord{\overline{A},B}$$


Remark:
\begin{itemize}
\item $(\overline{A},B)$ denotes the type $(A_1,A_2, \ldots, A_n, B)$;
\item all the types appearing in the rule are not required to be homogeneous. For instance
the type $(A,\ldots,A_l,B)$ in the rule $\rulename{app}$ may be such that $\ord{A_l} < \ord{B}$;
\item the environment $\Gamma \union \overline{x}:\overline{A}$ is not stratified. In particular, variables in $\overline{x}$ do not necessarily have the same order;
\item In the abstraction rule, the side-condition imposes that at least all the variable of the lowest order
in the context are abstracted. However other variables can also be
abstracted together with the lowest order variables. Moreover there
is not constraint on the order on which the variables are abstracted
(this contrasts with the homogeneous safe lambda calculus);
\end{itemize}

\begin{exmp}
Suppose $x:o$, $f:o\rightarrow o$ and $\varphi:(o\rightarrow
o)\rightarrow o$ then the term $$\vdash \lambda x f \varphi .
\varphi : o \rightarrow (o\rightarrow o) \rightarrow ((o\rightarrow
o)\rightarrow o) \rightarrow (o\rightarrow o)\rightarrow o$$ is
a valid non homogeneous safe term.
\end{exmp}

Side-remark: safety is preserved by $\eta$-expansion: consider the safe term
$\Gamma \vdash M:(A_1,\ldots,A_l,o)$ where $(A_1,\ldots,A_l,o)$ is not homogeneous. Then for all $i \in 1..l$ we have $\Gamma \union \Sigma \vdash x_i :A_i$ for some
context $\Sigma = \{ x_1:A_1, \cdots x_l :A_l \}$. Applying $\rulename{app}$ we then get that $\Gamma, \Sigma \vdash M x_1 \ldots x_l$ is valid. Hence
the $\eta$-expansion of $M$ is safe:
$$\Gamma \vdash \lambda x_1:A_1, \cdots x_l:A_l .\ M\ x_1 \ldots x_l$$


\begin{lem}[Context reduction]
\label{lem:nonhomosafe_basic_prop}
If $\Gamma \vdash M : B$ is a valid judgment then
\begin{enumerate}
\item $fv(M) \vdash M : B$
\item every variable in $\Gamma$ \emph{occuring free in $M$} has order at
least $ord(M)$.
\end{enumerate}
where $fv(M)$ denotes the context constituted of the free variables occurring in $M$.
\end{lem}
\begin{proof}
(i) Suppose some variable $x$ in $\Gamma$ does not occur free in $M$,
then the $x$ must have been introduced in the context by the weakening rule.
Hence $M$ must also be typable with the rules of the safe lambda calculus but with the variable $x$ removed from the context.
(ii) An easy structural induction.
\end{proof}

The converse of this lemma is not true: consider the simply typed term $\lambda y z. (\lambda x . y ) z$ with $x,y,z:o$. This term is closed therefore it satisfies
property (i) and (ii) of lemma \ref{lem:nonhomosafe_basic_prop}. However it is not typable by the rules of the safe lambda-calculus since the subterm
$\lambda x .y$ is not safe.

\subsection{Substitution in the safe lambda calculus}

The traditional notion of substitution, on which the
$\lambda$-calculus is based on, is defined as follows:
\begin{dfn}[Substitution]
\label{dfn:subst}
\begin{eqnarray*}
c \subst{t}{x} &=& c \quad \mbox{where $c$ is a $\Sigma$-constant}\\
x \subst{t}{x} &=& t\\
 y\subst{t}{x} &=& y \quad \mbox{for } x \not \neq y,\\
(M_1 M_2) \subst{t}{x} &=& (M_1 \subst{t}{x}) (M_2 \subst{t}{x})\\
(\lambda x . M) \subst{t}{x} &=& \lambda x . M\\
(\lambda y . M) \subst{t}{x} &=& \lambda z . M \subst{z}{y}
\subst{t}{x} \mbox{where $z$ is a fresh variable and $x\not = y$}
\end{eqnarray*}
\end{dfn}

In the setting of the safe lambda calculus, the notion of
substitution can be simplified. Indeed, similarly to what we observe in the homogeneous
safe $\lambda$-calculus, we remark that for safe
$\lambda$-terms there is no need to rename variables when performing
substitution:

\begin{lem}[No variable capture lemma]
\label{lem:noclash} There is no variable capture when performing
substitution on a safe term.
\end{lem}

This is the equivalent of lemma \ref{lem:homog_nocapture} for the non-homogeneous case. The proof (which does not rely on homogeneity)
is identical.
Consequently, in the safe lambda calculus setting, we can omit to to rename
variable when performing substitution and the equation
$$(\lambda x . M) \subst{t}{y} = \lambda z . M \subst{z}{x}
\subst{t}{y} \mbox{where $z$ is a fresh variable}$$ becomes
$$(\lambda x . M) \subst{t}{y} = \lambda x . M \subst{t}{y}.$$

Unfortunately, this notion of substitution is still not adequate for
the purpose of the safe simply-typed lambda calculus. The problem is
that performing a single $\beta$-reduction on a safe term will not
necessarily produce another safe term.

The solution consist in reducing several consecutive $\beta$-redex at the same time until we obtain a safe
term. To achieve this, we introduce the \emph{simultaneous substitution},
a generalization of the standard substitution given in definition \ref{dfn:subst}.

\begin{dfn}[Simultaneous substitution]
\label{dnf:simsubst}
 The expression $\subst{\overline{N}}{\overline{x}}$ is an abbreviation for $\subst{N_1 \ldots N_n}{x_1
\ldots x_n}$:
\begin{eqnarray*}
c \subst{\overline{N}}{\overline{x}} &=& c \quad \mbox{where $c$ is a $\Sigma$-constant}\\
x_i \subst{\overline{N}}{\overline{x}} &=& N_i\\
 y \subst{\overline{N}}{\overline{x}} &=& y \quad \mbox{ if } y \not \neq x_i \mbox{ for all } i,\\
(M N) \subst{\overline{N}}{\overline{x}} &=& (M \subst{\overline{N}}{\overline{x}}) (N \subst{\overline{N}}{\overline{x}}) \\
(\lambda x_i . M) \subst{\overline{N}}{\overline{x}} &=& \lambda x_i
. M
\subst{N_1 \ldots N_{i-1} N_{i+1}\ldots N_n}{x_1 \ldots x_{i-1} x_{i+1}\ldots x_n} \\
(\lambda y . M)
\subst{\overline{N}}{\overline{x}} &=& \lambda z . M \subst{z}{y} \subst{\overline{N}}{\overline{x}} \\
&& \mbox{where $z$ is a fresh variables and } y \neq x_i \mbox{ for
all } i
\end{eqnarray*}
\end{dfn}

In general, variable captures should be avoided, this explains why
the definition of simultaneous substitution uses auxiliary fresh
variables. However in the current setting, lemma \ref{lem:noclash}
can clearly be transposed to the simultaneous substitution therefore
there is no need to rename variable.

The notion of substitution that we need is therefore the
\emph{capture permitting simultaneous substitution} defined as
follow:

\begin{dfn}[Capture permitting simultaneous substitution]
 We use the notation
$\subst{\overline{N}}{\overline{x}}$ for $\subst{N_1 \ldots N_n}{x_1
\ldots x_n}$:
\begin{eqnarray*}
c \subst{\overline{N}}{\overline{x}} &=& c \quad \mbox{where $c$ is a $\Sigma$-constant}\\
 x_i \subst{\overline{N}}{\overline{x}} &=& N_i\\
 y \subst{\overline{N}}{\overline{x}} &=& y \quad \mbox{where } x \not \neq y_i \mbox{ for all } i,\\
(M_1 M_2) \subst{\overline{N}}{\overline{x}} &=& (M_1 \subst{\overline{N}}{\overline{x}}) (M_2 \subst{\overline{N}}{\overline{x}})\\
(\lambda x_i . M) \subst{\overline{N}}{\overline{x}} &=& \lambda x_i
. M
\subst{N_1 \ldots N_{i-1} N_{i+1}\ldots N_n}{x_1 \ldots x_{i-1} x_{i+1}\ldots x_n} \\
(\lambda y . M) \subst{\overline{N}}{\overline{x}} &=& \lambda y . M
\subst{\overline{N}}{\overline{x}} \mbox{where $y \not = x_i$ for
all $i$} \qquad \mathbf{(\star)}
\end{eqnarray*}
The symbol $\mathbf{(\star)}$ identifies the equation that changed
compared to the previous definition.
\end{dfn}

\begin{lem}[Substitution preserves safety]
\label{lem:subst_preserve_i}
$$ \Gamma\union \overline{x} : \overline{A}\vdash M : T
\quad \mbox{and} \quad \Gamma \vdash N_k : B_k \mbox{, } k \in
1..n \qquad \mbox{ implies } \qquad \Gamma \vdash
M[\overline{N}/\overline{x}] : T$$
\end{lem}

\begin{proof}
Suppose that $\Gamma \union \overline{x}: \overline{A} \vdash M :T$ and
$\Gamma \vdash N_k : B_k$ for $k \in 1..n$.

We prove $\Gamma \vdash M[\overline{N}/\overline{x}]$ by induction
on the size of the proof tree of $\Gamma\union \overline{x}:\overline{A}
\vdash M : T$ and by case analysis on the last rule used. We just
give the detail for the abstraction case. Suppose that the property
is verified for terms whose proof tree is smaller than $M$. Suppose
$\Gamma \union \overline{x}:\overline{A} \vdash \lambda \overline{y} :
\overline{C}. P : (\overline{C}|D)$ where $\Gamma\union
\overline{x}:\overline{A}\union \overline{y}:\overline{C} \vdash P :
D$, then by the induction hypothesis $\Gamma\union
\overline{y}:\overline{C} \vdash
P\subst{\overline{N}}{\overline{x}} : D$. Applying the rule
$\rulename{abs}$ gives $\Gamma \vdash \lambda
\overline{y}:\overline{C} . P \subst{\overline{N}}{\overline{x}}$.
\end{proof}

\subsection{Safe-redex}
In the simply-typed lambda calculus a redex is a term of the form
$(\lambda x . M) N$. We generalize this definition to the safe
lambda calculus:
\begin{dfn}[Safe redex]
We call safe redex a term of the form $(\lambda \overline{x} . M)
N_1 \ldots N_l$ such that:
\begin{itemize}
\item $ \Gamma \vdash (\lambda \overline{x} . M) N_1 \ldots N_l $
\item the variable $\overline{x}=x_1\ldots x_n$ are abstracted altogether by one occurrence of the rule $\rulename{abs}$ in the proof tree.
\item The terms $(\lambda \overline{x} . M)$, $N_1$, $N_l$ are applied together at once using the $\rulename{app}$ rule :
$$   \rulef{
            \Sigma \vdash \lambda \overline{x} . M
            \quad
            \Sigma \vdash N_1         \quad \ldots \quad \Sigma \vdash N_l
    }
    {
       \Sigma \vdash (\lambda \overline{x} . L) N_1 \ldots N_l
    } (\mathbf{app})
$$
Consequently each $N_i$ is safe.

\item $l\leq n$
\end{itemize}
\end{dfn}

Note that the condition $l\leq n$ in the definition is not too
restrictive since whenever $l>n$ it means that the application rule is ``wider'' than the abstration
therefore it can be replaced by an application of exactly $n$ terms
followed by another application for the remaining terms $N_{n+1},
\ldots, N_l$.


The relation $\beta_s$ is defined on safe-redex: $(s\mapsto t) \in \beta_s$ iff $s \equiv (\lambda \overline{x} . M) N_1 \ldots N_l$ is a safe redex and
$t \equiv \lambda x_l \ldots x_n . M \subst{N_1 \ldots N_l}{x_1 \ldots x_l}$.
The safe $\beta$-reduction noted $\betasred$ is the closure of the relation $\beta_s$ by compatibility with the formation rules of the safe $\lambda$-calculus.
As we did in the homogeneous case, it is straightforward to show that $\betasred \subseteq \betared^*$.


\begin{lem}
\label{lem:safereduction} A safe redex reduces to a safe term.
\end{lem}

This lemma, which is a consequence of lemma \ref{lem:subst_preserve_i}, is the counterpart of lemma \ref{lem:homoh_safered_preserve_safety} in the homogeneous safe lambda calculus.
Their proofs are identical.


\subsection{Particular case of homogeneously-safe lambda terms}

In this section, we will refine the rules of the non-homogenous safe lambda calculus to the homogeneous case.

We recall the definition of type homogeneity given in section \ref{sec:homotypes}:
a type $(A_1, A_2, \ldots A_n, o)$ is said to be homogeneous whenever $\ord{A_1} \geq \ord{A_2} \geq
\ldots \geq  \ord{A_n}$ and each of the $A_i$ are homogeneous. A term is said homogeneous if its type is homogeneous.

Safety in the sense of Knapik et al. (\cite{KNU02}) is defined for homogeneous recursion scheme.
A recursion scheme is homogeneous if
\begin{itemize}
    \item[(i)] the $\Sigma$ constants are of order 1 at most and therefore have homogeneous types;
    \item[(ii)] the variables in the alphabet $\Delta$ have homogeneous types,
    \item[(iii)] and every non-terminal in the recursion scheme has a homogeneous type.
\end{itemize}

We now impose the same restrictions on the terms generated by our system rules.
The first and second restriction imposes that every applicative terms in $\mathcal{T}(\Delta)$ must be homogeneous.

Abstractions in simply-typed terms correspond to non-terminals in recursion schemes,
therefore by imposing restriction (iii) to our calculus, all the sequents generated by the rules must be of homogeneous type.
We say that a term is \emph{homogeneously-safe} if its type is homogeneous
and there is a proof tree showing its safety where all the sequents
of the proof tree are of homogenous type.

We say that $\Gamma \vdash M : A$ verifies $P_i$ for $i \in \zset$ if all the
variables in $\Gamma$ have orders at least $\ord{A}+i$.
Lemma \ref{lem:nonhomosafe_basic_prop} can then be restated as follows:

\begin{lem}[Context reduction]
\label{lem:context_reduction} If $\Gamma \vdash M : A$ then the sequent $fv(M) \vdash M : A$ is valid and satisfies $P_0$.
\end{lem}


We now prove that if we impose the homogeneity of types, the set of rules of the non-homogenous safe $\lambda$-calculus
and the rules of table \ref{tab:homosafelmd_rules_refined} are equivalent.  We recall that in the system of rules of
table \ref{tab:homosafelmd_rules_refined}, if the sequent $\Gamma \vdash^{i} M : A$ is valid for some $i \in
\zset$ then all the variables in $\Gamma$ have orders at least $\ord{A}+i$.

\begin{prop}[Homogeneity restriction]
\label{prop:nonhomogsafe_homog_restriction}
Let $k \in \{ 0, -1 \}$. The sequent $\Gamma \vdash M : A$ is valid, homogeneously-safe and satisfies $P_k$
if and only if the sequent $\Gamma \vdash^k M : A$ is valid in the system of rules of table \ref{tab:homosafelmd_rules_refined}.
\end{prop}

\begin{proof}
\emph{If}: An easy induction by case analysis on the last rule used to derive $\Gamma \vdash^0 M : A$.

\emph{Only if}:
Consider an homogeneously-safe term $\Gamma \vdash S : T$ satisfying $P_0$.
We proceed by induction and case analysis on the last rule used to derive $\Gamma \vdash S : T$.
We only give the details for the application and abstraction
case:
\begin{itemize}
\item \textbf{Abstraction.} We recall the abstraction rule:
$$ \rulename{abs} \quad  \rulef{\Gamma \union \overline{x} : \overline{A} \vdash M : B}
                                   {\Gamma  \vdash \lambda \overline{x} : \overline{A} . M : (\overline{A},B)} \qquad
                                   \forall y \in \Gamma : \ord{y} \geq \ord{\overline{A},B}$$

Type homogeneity requires that for all $i$: $\ord{x_i} = \ord{A_i} \geq
\ord{B} -1$. Therefore the premise of the rule verifies $P_{-1}$. Using the induction hypothesis we have:
\begin{equation}
\Gamma \union \overline{x} : \overline{A} \vdash^{-1} M : B. \label{eq:prop:nonhomogsafe_homog_restriction:abs1}
\end{equation}

We now partition the context $\Gamma$ according to the order of
the variables. The partitions are written in decreasing order of
type order. The notation $\Gamma | \overline{x}:\overline{A}$ means
that $\overline{x}:\overline{A}$ is the lowest partition of the
context.
We also use the notation $(\overline{A}|B)$ to denote the
homogeneous type $(A_1, A_2, \ldots A_n, B)$ where $\ord{A_1} =
\ord{A_2} =  \ldots \ord{A_n} \geq \ord{B} -1$.


Suppose that we abstract a single variable $x$,
then in order to respect the side condition, we need to abstract all
variables of order lower or equal to $\ord{x}$. In particular we
need to abstract the partition of the order of $x$.
Moreover to respect type homogeneity, we need to abstract variables
of the lowest order first.

Hence $\overline{x}$ must contain at least the lowest variable partition (all the variables of the lowest order).
If $\overline{x}$ contains variables of different order, then the instance of the abstraction rule can be replaced by consecutive
instances of the abstraction rule, one for each of the different order of variable present in $\overline{x}$.
Therefore, without loose of generality, we can assume that $\overline{x}$ only contains the lowest partition, that is to say,
$\overline{x}$ \emph{is} the lowest partition.

The sequent \ref{eq:prop:nonhomogsafe_homog_restriction:abs1} therefore becomes:
$$\Gamma | \overline{x} : \overline{A} \vdash^{-1} M : B.$$

And we can conclude by applying the abstraction rule of table \ref{tab:homosafelmd_rules_refined}:
$$ \rulename{abs} \quad  \rulef{\Gamma| \overline{x} : \overline{A} \vdash^{-1} M : B}
                                   {\Gamma  \vdash^{0} \lambda \overline{x} : \overline{A} . M : (\overline{A}|B)}$$



\item \textbf{Application.} We recall the application rule:
$$ \rulename{app} \  \rulef{\Gamma \vdash M : (A,\ldots,A_l,B)
                                        \qquad \Gamma \vdash N_1 : A_1
                                        \quad \ldots \quad \Gamma \vdash N_l : A_l  }
                                   {\Gamma  \vdash M N_1 \ldots N_l : B}
                                    \quad
                                   \forall y \in \Gamma : \ord{y} \geq \ord{B}$$

The term in the conclusion is homogeneously safe therefore the term in the first premise must be of homogeneous \
type. This implies that $\ord{A_1} \geq \ldots \geq \ord{A_l}
\geq \ord{B} - 1$.
Furthermore, we can make the assumption that $\ord{A_1} = \ldots = \ord{A_l} = \ord{\overline{A}}$
(it is always possible to replace an instance of the application rule
by several consecutive instances of this kind).

By lemma \ref{lem:context_reduction}, we have for all $i \in 1..l$:
$$fv(N_i) \vdash N_i : A_i \mbox{ is valid and satisfies } P_0.$$

Let $\Sigma = \Union_{i=1..p} fv(N_i)$. Since $\ord{A_1} = \ldots = \ord{A_l}$, by applying the weakening rule we get for all $i\in 1..p$:
$$\Sigma \vdash N_i : A_i \mbox{ is valid and satisfies } P_0.$$


Applying lemma \ref{lem:context_reduction} to the term $M$ we have:
$$fv(M) \vdash M : (A_1,\ldots,A_l,B) \mbox{ is valid and satisfies } P_0.$$

The weakening rule $\rulename{wk}$ then gives:
$fv(M) \union \Sigma \vdash M : (A_1,\ldots,A_l,B)$.
Since $\Sigma \vdash N_i : A_i$ satisfies $P_0$, for any
$z \in \Sigma$ we have $\ord{z} \geq \ord{A_i} = \ord{(A_1,\ldots,A_l,B)} - 1$.
Hence:
\begin{equation}
fv(M) \union \Sigma \vdash M : (A_1,\ldots,A_l,B) \mbox{ is valid and satisfies } P_{-1} \label{eq:prop:nonhomogsafe_homog_restriction:m}
\end{equation}

Similarly, for all $i \in 1..p$, the weakening rule gives $fv(M) \union \Sigma \vdash N_i : A_i$.
Since $fv(M) \vdash M : (A_1,\ldots,A_l,B)$ satisfies $P_0$,
for any $z \in fv(M)$ we have $\ord{z} \geq \ord{M} \geq \ord{A_i}$. Hence:
\begin{equation}
fv(M) \union \Sigma \vdash N_i : A_i \mbox{ is valid and satisfies } P_0 \label{eq:prop:nonhomogsafe_homog_restriction:ni}
\end{equation}

Let us define the context $\Sigma' = fv(M) \union \Sigma$. Using the induction hypthesis on equation
\ref{eq:prop:nonhomogsafe_homog_restriction:m} and \ref{eq:prop:nonhomogsafe_homog_restriction:ni} we have:
$$
\Sigma' \vdash^{-1} M : (A_1,\ldots,A_l,B) \qquad \mbox{and} \qquad \Sigma' \vdash^0 N_i : A_i \mbox{ for all } i \in 1..l
$$


We consider the following two sub-cases:
\begin{itemize}
\item If $A_1, \ldots A_l$ forms a type partition then we can apply
rule $\rulename{app}$ of table \ref{tab:homosafelmd_rules_refined}:

$$ \rulef{\Sigma' \vdash^{-1} M : \overline{A} | B
                                        \qquad \Sigma' \vdash^{0} N_1 :
                                        A_1
                                        \quad \ldots \quad \Sigma' \vdash^{0} N_l :
                                        A_l
                                        \quad l = |\overline{A}|
                                        }
                                   {\Sigma'  \vdash^{0} M N_1 \ldots N_l : B} \quad  \rulename{app}
$$
where $\overline{A} = A_1, \ldots A_l$.

\item  Suppose that $A_1, \ldots A_l$ do not form a type partition, then we
have $$\ord{A_1} = \ldots = \ord{A_l} = \ord{B} - 1.$$

The side condition in the original instance of the application rule says:
$$\forall y \in \Gamma : \ord{y} \geq \ord{B} = 1 + \ord{A_l} = \ord{(A_1,\ldots, A_l,B)} = \ord{M}$$

In particular the variables in $\Sigma' \subseteq \Gamma$ are of order greater than $\ord{M}$ and consequently
the sequent $\Sigma' \vdash M : (A,\ldots,A_l,B)$ verifies $P_0$. The induction hypothesis then gives:
$$\Sigma' \vdash^0 M : (A,\ldots,A_l,B)$$

By using $l$ consecutive instances of the rules $\rulename{app^+}$ from table \ref{tab:homosafelmd_rules_refined} we get:
$$  \rulef{ \rulef{ \rulef{ \Sigma' \vdash^0 M : (A_1,\ldots, A_l,B)
                    \qquad \Sigma'\vdash^{0} N_1 : A_1
                    }{ \Sigma' \vdash^0 M N_1 : (A_2,\ldots, A_l,B)} \quad \rulename{app^+}
          }
          { \vdots
          }
          \quad \rulename{app^+}
       }
       { \Sigma'  \vdash^{0} M N_1 \ldots N_l : B } \quad \rulename{app^+}
$$
\end{itemize}

In both cases we have proved that $\Sigma'  \vdash^{0} M N_1 \ldots N_l : B$ is a valid sequent.

Clearly $\Sigma' \subseteq \Gamma$ since $fv(M) \subseteq \Gamma$ and $\Sigma' = \Union_{i\in1..l} fv(N_i) \subseteq \Gamma$.
Suppose that $\Sigma' = \Gamma$ then the proof is done.
Suppose that $\Sigma' \subset \Gamma$, then the side condition in the original instance of the application rule says that all
the variables in $\Gamma$ have order
greater or equal to $\ord{B}$, we can therefore apply the weakening rule $\rulename{wk^0}$
of table \ref{tab:homosafelmd_rules_refined} exactly $|\Gamma\setminus \Sigma'|$ times and get:
$$ \rulef{\Sigma'  \vdash^{0} M N_1 \ldots N_l : B}
                                   {\Gamma  \vdash^{0} M N_1 \ldots N_l : B} \quad \rulename{wk^0}
$$


\end{itemize}
\end{proof}


\subsection{Examples}
\subsubsection{Example 1}
Let $f,g:o\rightarrow o$, $x,y:o\rightarrow o$, $\Gamma =
g:o\rightarrow o$ and $\Gamma' = g:o\rightarrow o, y:o$. The term
$(\lambda f x . x) g y $ is safe. One possible proof tree is:
$$ \rulef{
        \rulef{
            \rulef{
                \rulef{\vdots}{\Gamma \vdash \lambda f x. x}      \qquad \axiomf{\Gamma \vdash g} }
            {\Gamma \vdash (\lambda f x. x) g} \rulename{app}
        }
        { \Gamma' \vdash (\lambda f x. x) g } \rulename{wk}
        \qquad \axiomf{\Gamma' \vdash y}
    }
    { \Gamma' \vdash (\lambda f x. x) g y } \rulename{app}
$$
Here is another proof for the same judgment:
$$ \rulef{  \rulef{ \rulef{\vdots}{\Gamma \vdash \lambda f x. x} }{\Gamma' \vdash \lambda f x. x} \rulename{wk}    \qquad \rulef{}{\Gamma' \vdash g} \qquad \rulef{}{\Gamma' \vdash y}}
    {\Gamma' \vdash (\lambda f x. x) g y } \rulename{app}$$

We see on this particular example that there may exist different
proof trees deriving the same judgment.

\subsubsection{Example 2 - Damien Sereni SCT counter-example}
In \cite{serenistypesct05}, the following counter-example is given
to show that not all simply-typed terms are size-change terminating
(see \cite{jones01} for a definition of size-change termination):

$$ E =  (\lambda a . a (\lambda b . a (\lambda c d .d))) (\lambda e . e (\lambda f .f))$$
where:
\begin{eqnarray*}
a &:& \sigma \typear \mu \typear \mu \\
b &:& \tau \typear \tau \\
c &:& \tau \typear \tau \\
d &:& \mu \\
e &:& \sigma = (\tau \typear \tau) \typear \mu \typear \mu \\
f &:& \tau
\end{eqnarray*}
and $\tau$, $\mu$ and $\sigma$ are type variables.

This example shows that the safe $\lambda$-calculus with no
homogeneity restriction that we have defined at the beginning of
this section generates a class of terms that strictly contains the
terms typable in the homogeneous safe $\lambda$-calculus of section
\ref{sec:safe_homog}.

Indeed, for $E$ to be an homogeneous safe lambda term, in the sense
of the rules of section \ref{sec:safe_homog}, $\tau$ and $\mu$ must
be homogeneous types and the variables $a,b,c,d,e,f$ must be
homogeneously typed. This implies that:
$$ \ord{\tau} \geq \ord{\mu}-1$$
Conversely, if this condition is met then $\vdash E : \mu \typear
\mu$ is a valid judgement of the \emph{homogeneous} safe
$\lambda$-calculus.

However with the rules of the \emph{type-unrestricted} safe
lambda-calculus, the term $E$ is always safe for any type $\mu$ and
$\tau$.
